formulate metaspecification, TODO induction

examples/contractMorphisms/specifyUpgrade/upgrade.v
@@ -22,7 +22,7 @@ Open Scope string.
 
 (** Example 5.3.1: 
     This example recalls the Uranium Finance hack of 2021 due to an incorrect upgrade:
-    A constant `k` was changed from 1_000 to 1_000_000 in all but one of its instances 
+    A constant `k` was changed from 1_000 to 10_000 in all but one of its instances 
     in the contract.
 
     This example illustrates how a contract upgrade can be *specified* using contract 
@@ -46,8 +46,10 @@ Context { storage : Type } `{ storage_ser : Serializable storage }
         { other_entrypoint : Type }.
 
 (** We assume that entrypoint type includes a trade function, among other entrypoints. *)
+Context { trade_data : Type } { trade_qty : trade_data -> N }.
+
 Class Msg_Spec (T : Type) := {
-    trade : N -> T ; 
+    trade : trade_data -> T ; 
     (* for any other entrypoint types *)
     other : other_entrypoint -> option T ;
 }.
@@ -77,18 +79,18 @@ Context { C : Contract setup entrypoint storage error }.
 
 (** such that get_bal changes according to calculate_trade, meaning that: *)
 Definition spec_trade : Prop :=
-    forall cstate chain ctx qty cstate' acts,
+    forall cstate chain ctx trade_data cstate' acts,
     (** for any successful call to the trade entrypoint of C, *)
-    receive C chain ctx cstate (Some (trade qty)) = Ok(cstate', acts) -> 
+    receive C chain ctx cstate (Some (trade trade_data)) = Ok(cstate', acts) -> 
     (** the balance in storage updates as follows. *)
     get_bal cstate' = 
-    get_bal cstate + calculate_trade qty.
+    get_bal cstate + calculate_trade (trade_qty trade_data).
 
 Context { spec_trade : Prop }.
 
 (** Now suppose that we have another calculate_trade function, this time which calculates 
-    trades at three more digits of precision. *)
-Definition round_down (n : N) := n / 1_000.
+    trades at one more digit of precision. *)
+Definition round_down (n : N) := n / 10.
 
 Context { calculate_trade_precise : N -> N }
     (** (i.e. calculate_trade_precise rounds down to calculate_trade) *)
@@ -105,12 +107,12 @@ Context { C' : Contract setup entrypoint storage error }.
 
 (** but now trades are calculated in line with calculate_trade_precise. *)
 Definition spec_trade_precise : Prop :=
-    forall cstate chain ctx qty cstate' acts,
+    forall cstate chain ctx trade_data cstate' acts,
     (** ... meaning that for a successful call to the trade entrypoint of C', *)
-    receive C' chain ctx cstate (Some (trade qty)) = Ok(cstate', acts) -> 
+    receive C' chain ctx cstate (Some (trade trade_data)) = Ok(cstate', acts) -> 
     (** the balance held in storage goes up by calculate_trade_precise. *)
     get_bal cstate' = 
-    get_bal cstate + calculate_trade_precise qty.
+    get_bal cstate + calculate_trade_precise (trade_qty trade_data).
 
 Context { spec_trade_precise : Prop }.
 
@@ -120,19 +122,24 @@ Context { spec_trade_precise : Prop }.
 
 (** 1. f rounds trades down when it maps inputs *)
 Definition f_recv_input_rounds_down (f : ContractMorphism C' C) : Prop := 
-    forall c ctx st e t,
-    (*  *)
-    e = trade t -> 
-    (*  *)
-    recv_inputs C' C (recv_cm f) (c, ctx, st, (Some e)) = 
-    (c, ctx, state_morph st, Some (trade (round_down t))).
+    forall c ctx st e e' t',
+    (* for calls to the TRADE entrypoint *)
+    e' = trade t' -> 
+    (* then in the mapping by f, *)
+    recv_inputs C' C (recv_cm f) (c, ctx, st, Some e') = 
+    (c, ctx, state_morph st, Some e) -> 
+    (* f sends trades to trades, *)
+    exists t,
+    e = trade t /\
+    (* such that the trade_qty of t is the rounded-down trade_qty of t' *)
+    trade_qty t = round_down (trade_qty t').
 
 (** 2. aside from trade, f doesn't touch the other entrypoints *)
 Definition f_recv_input_other_equal (f : ContractMorphism C' C) : Prop := 
     forall e o,
-    (*  *)
+    (* for calls to all other entrypoints, *)
     e = other o ->
-    (*  *)
+    (* f is the identity *)
     recv_inputs C' C (recv_cm f) = id.
 
 (** 3. f rounds down on the storage, but doesn't touch anything else. *)
@@ -165,17 +172,42 @@ Definition upgrade_spec (f : ContractMorphism C' C) : Prop :=
 
 
 (** The Upgrade Metaspecification.
-    To justify that upgrade_spec actually specifies a correct upgrade, we prove the following
-    result(s). *)
+    To justify that upgrade_spec actually specifies a correct upgrade, we prove 
+    the following result(s). *)
 
 (*** Suppose there exists some f : C' -> C satisfying upgrade_spec. *)
 Context { f : ContractMorphism C' C } { is_upgrade_morph : upgrade_spec f }.
 
+(*  *)
+Definition morphism_lift (caddr : Address) : ChainState -> ChainState. Admitted.
+(* sends *)
+Theorem morphism_lift_commutes : forall bstate' caddr cstate',
+    (* bstate' is reachable *)
+    reachable bstate' ->
+    (* where C' is at caddr with state cstate' *)
+    env_contracts bstate' caddr = Some (C' : WeakContract) -> 
+    contract_state bstate' caddr = Some cstate' ->
+    (*  *)
+    let bstate := morphism_lift caddr bstate' in  
+    let cstate := state_morph cstate' in 
+    env_contracts bstate caddr = Some (C : WeakContract) /\
+    contract_state bstate caddr = Some cstate.
+Admitted.
 
-(** Then (TODO) A property that formalizes "does the same but different" *)
-
-
-
-
+(* All states of C' relate to equivalent states of C by rounding down *)
+Theorem rounding_down_invariant bstate' caddr :
+    (* Forall reachable states with contract at caddr, *)
+    reachable bstate' -> 
+    env_contracts bstate' caddr = Some (C' : WeakContract) ->
+    let bstate := morphism_lift caddr bstate' in  
+    (* cstate is the state of the contract AND *)
+    exists (cstate' cstate : storage),
+    contract_state bstate' caddr = Some cstate' /\
+    contract_state bstate caddr = Some cstate /\
+    (* such that for cstate, the state of C in bstate, 
+        the balance in cstate is rounded-down from the balance of cstate' *)
+    get_bal cstate = round_down (get_bal cstate').
+Admitted.
+    (* goal : use contract induction *)
 
 End UpgradeSpec.
